proof/correctness/Correctness_XMSS.ec
@@ -18,6 +18,33 @@ require import BitEncoding.
 
 require import Termination.
 
+clone import DListProgramX as T
+  with type t <- W8.t,
+       op d <- W8.dword.
+
+lemma size_W32toBytes (x : W32.t) : size (W32toBytes x) = 4 
+    by rewrite /W32toBytes size_map size_chunk //.
+
+lemma W32toBytes_zero_nth (i : int) :
+    0 <= i < 4 => nth witness (W32toBytes W32.zero) i = W8.zero.
+proof.
+move => H.
+rewrite /W32toBytes.
+case (i = 0).
+  + move => ?; admit.
+case (i = 1).
+  + move => ??; admit.
+case (i = 2).
+  + move => ???; admit.  
+move => ???.
+rewrite (: i = 3) 1:/#.
+have ->: w2bits W32.zero = nseq 32 false. 
+  + rewrite /w2bits. apply (eq_from_nth witness); [ by rewrite size_mkseq size_nseq |].   
+    rewrite size_mkseq (: max 0 32 = 32) 1:/# => j Hj.
+    rewrite nth_nseq //= nth_mkseq //=.
+admit.
+qed.
+
 (*** Treehash kg ***)
 
 lemma treehash_kg_correct :
@@ -35,11 +62,6 @@ qed.
 
 (*** Key Gen ***)
 
-clone import DListProgramX as T
-  with type t <- W8.t,
-       op d <- W8.dword.
-
-
 lemma random_bytes_equiv :
     n = XMSS_N =>
     equiv [
@@ -56,6 +78,7 @@ transitivity {2} { pub_seed <$ dlist W8.dword 96; }
 (true ==> pub_seed{1} = (sk_seed{2} ++ sk_prf{2} ++ pub_seed{2}) ) => //.
   + rnd Array96.to_list (Array96.of_list W8.zero): *0 *0.
     auto => />; split => [l | ?].
+
       * rewrite supp_dmap; move => [x].
         rewrite supp_dlist // => /> E _.
         by rewrite of_listK.
@@ -110,7 +133,6 @@ proof.
 admit.
 qed.
 
-
 (*** Keygen without OID ***)
 lemma xmss_kg_no_oid : 
     n = XMSS_N /\ 
@@ -119,8 +141,8 @@ lemma xmss_kg_no_oid :
       M(Syscall).__xmssmt_core_keypair ~ XMSS_MT_PRF.kg :
       true 
       ==>
-      res{2}.`1 = EncodeSkNoOID res{1}.`2 /\
-      res{2}.`2 = EncodePkNoOID res{1}.`1
+      res{1}.`1 = DecodePkNoOID res{2}.`2 /\
+      res{1}.`2 = DecodeSkNoOID res{2}.`1
     ].
 proof.
 rewrite /XMSS_N /XMSS_D => [#] *. 
@@ -133,44 +155,42 @@ seq 1 1 : (
   size sk_prf{2} = 32 /\
   size pub_seed{2} = 32 
 ); first by call random_bytes_results => //=; skip => /> /#.
-
-
-
-
-
-
-
-
-
-
-
-
-
-
 inline {1} M(Syscall).__xmssmt_core_seed_keypair. 
 seq 12 0 : (#pre /\ pk0{1} = pk{1} /\  sk0{1} = sk{1} /\ seed0{1} = seed_p{1}); first by auto. 
+seq 0 0 : (
+  #pre /\
+  (forall (k : int), 0 <= k < 32 => seed_p{1}.[k] = nth witness sk_seed{2} k) /\
+  (forall (k : int), 0 <= k < 32 => seed_p{1}.[32+k] = nth witness sk_prf{2} k) /\
+  (forall (k : int), 0 <= k < 32 => seed_p{1}.[64+k] = nth witness pub_seed{2} k)
+).
+    + auto => /> &1 &2 H0 H1 H2 H3; do split => k??. 
+        * rewrite -get_to_list H0 nth_cat !size_cat H1 H2 ifT 1:/# nth_cat H1 ifT //=.
+        * rewrite -get_to_list H0 nth_cat !size_cat H1 H2 ifT 1:/# nth_cat H1 ifF /#.
+        * rewrite -get_to_list H0 nth_cat !size_cat H1 H2 ifF /#.  
 seq 1 1 : (#pre /\ address{2} = top_tree_addr{1}).
-    + (* exists * top_tree_addr{1}; elim * => _P; call {1} (zero_addr_op_impl _P). *) (* FIXME: TODO: This should work but I get a invalid goal shape *)
-      inline {1}; wp; sp. 
-      while {1} (0 <= i{1} <= 8 /\ forall (k : int), 0 <= k < i{1} => addr0{1}.[k] = W32.zero) (8 - i{1}).
-         * auto => /> *; do split;1,2,4:smt(); move => k??; rewrite get_setE /#.
-         * skip => /> *; split; [smt() |]; move => *; split; [smt() | move => ????; rewrite /zero_address; smt(@Array8)].
+    + inline M(Syscall).__zero_address_; wp; sp.
+      exists * top_tree_addr{1}; elim * => _P. 
+      call {1} (zero_addr_res _P); auto. (* NOTE: This requires zero_addr to be phoare because on the right hand side we have an operator and on the left hand side we have a procedure call *)
 seq 1 1 : (#pre); first by inline {1}; auto => /> *; rewrite /set_layer_addr /#. 
 seq 2 0 : (#pre /\ to_list idx{1} = nseq 4 W8.zero).
     + call {1} memset_nseq; auto. 
 seq 1 0 : (
-                 to_list seed_p{1} = sk_seed{2} ++ sk_prf{2} ++ pub_seed{2} /\
-                 size sk_seed{2} = 32 /\ 
-                 size sk_prf{2} = 32 /\ 
-                 size pub_seed{2} = 32 /\
-                 pk0{1} = pk{1} /\ 
-                 seed0{1} = seed_p{1} /\
-                 address{2} = top_tree_addr{1} /\
-                 to_list idx{1} = nseq 4 W8.zero /\
-                 forall (k : int), 0 <= k < 4 => sk0{1}.[k] = W8.zero
+  to_list seed_p{1} = sk_seed{2} ++ sk_prf{2} ++ pub_seed{2} /\
+  size sk_seed{2} = 32 /\ 
+  size sk_prf{2} = 32 /\ 
+  size pub_seed{2} = 32 /\
+  pk0{1} = pk{1} /\ 
+  seed0{1} = seed_p{1} /\
+  address{2} = top_tree_addr{1} /\
+  to_list idx{1} = nseq 4 W8.zero /\
+  (forall (k : int), 0 <= k < 4 => sk0{1}.[k] = W8.zero) /\
+  (forall (k : int), 0 <= k < 32 => seed_p{1}.[k] = nth witness sk_seed{2} k) /\
+  (forall (k : int), 0 <= k < 32 => seed_p{1}.[32+k] = nth witness sk_prf{2} k) /\
+  (forall (k : int), 0 <= k < 32 => seed_p{1}.[64+k] = nth witness pub_seed{2} k)
+
 ).
-    + auto => /> &1 &2 ???? H. 
-      have E : forall (k : int), 0 <= k < 4 => nth witness (to_list idx{1}) k = W8.zero by apply (nseq_nth (to_list idx{1}) 4 W8.zero);assumption.
+    + auto => /> &1 &2 ???? H???. 
+      have E : forall (k : int), 0 <= k < 4 => nth witness (to_list idx{1}) k = W8.zero by apply (nseq_nth (to_list idx{1}) 4 W8.zero); assumption.
       move => k??; rewrite initiE 1:/#; auto => />; rewrite ifT 1://=.
       rewrite -get_to_list; apply E => //.
 seq 2 0 : (
@@ -178,23 +198,9 @@ seq 2 0 : (
   forall (k : int), 0 <= k < 64 => buf1{1}.[k] = seed_p{1}.[k]
 ); first by auto => /> *; smt(@Array64).
 seq 1 0 : (#pre /\ buf0{1} = buf1{1}); first by ecall {1} (_x_memcpy_u8u8_64_post buf1{1}); skip => />. 
-seq 1 0 : (
-  #pre /\ 
-  forall (k : int), 0 <= k < 64 => sk0{1}.[4 + k] = seed0{1}.[k]
-); first by auto => /> *; split; move => ???; rewrite initE ifT 1:/#; auto => />; [rewrite ifF /# | rewrite ifT /#]. 
-seq 2 0 : (
-  #pre /\
-  forall (k : int), 0 <= k < 32 => bufn1{1}.[k] = seed_p{1}.[64 + k]
-); first by auto => /> *; smt(@Array32).
-seq 1 0 : (#pre /\ bufn0{1} = bufn1{1}); first by ecall {1} (_x_memcpy_u8u8_post bufn1{1}); skip => />. 
-seq 1 0 : (
-    #pre /\
-    forall (k : int), 0 <= k < 32 => sk0{1}.[4 + 3 *32 + k] = seed_p{1}.[64 + k]
-); first by auto => /> *; do split; move => *; rewrite initE ifT 1:/#; auto => />; [| | rewrite ifT /#]; rewrite ifF /#. 
 
-(* -------------------------------------------------------------------------------------------------------------------------------- *)
-(* Cleanup pre *)
-seq 0 0 : (
+(* At this point were in memcpy(sk, seed, 2 * params->n); *)
+seq 1 0 : (
   to_list seed_p{1} = sk_seed{2} ++ sk_prf{2} ++ pub_seed{2} /\
   size sk_seed{2} = 32 /\
   size sk_prf{2} = 32 /\
@@ -202,72 +208,133 @@ seq 0 0 : (
   pk0{1} = pk{1} /\
   seed0{1} = seed_p{1} /\
   address{2} = top_tree_addr{1} /\
-  to_list idx{1} = nseq 4 W8.zero /\
-        
 
-  (forall (k : int), 0 <= k <  4 => sk0{1}.[k] = W8.zero) /\ (* index *)
-  (forall (k : int), 0 <= k < 64 => sk0{1}.[4 + k] = seed_p{1}.[k]) /\ (* sk seed & sk prf *)
-  (forall (k : int), 0 <= k < 32 => sk0{1}.[4 + 3 * 32 + k] = seed_p{1}.[64 + k]) (* pub seed *)
-); first by auto => />. 
-(* -------------------------------------------------------------------------------------------------------------------------------- *)
+  (forall (k : int), 0 <= k < 32 => seed_p{1}.[k] = nth witness sk_seed{2} k) /\
+  (forall (k : int), 0 <= k < 32 => seed_p{1}.[32 + k] = nth witness sk_prf{2} k) /\
+  (forall (k : int), 0 <= k < 32 => seed_p{1}.[64 + k] = nth witness pub_seed{2} k) /\
+
+  to_list idx{1} = nseq 4 W8.zero /\
+
+  (forall (k : int), 0 <= k < 4 => sk0{1}.[k] = W8.zero) /\
+  (forall (k : int), 0 <= k < 32 => sk0{1}.[4 + k] = nth witness sk_seed{2} k) /\
+  (forall (k : int), 0 <= k < 32 => sk0{1}.[4 + 32 + k] = nth witness sk_prf{2} k)
+).
+    + auto => /> &1 &2 H0 H1 H2 H3 H4 H5 H6 H7 H8 H9; do split => k ??.
+        * rewrite initiE 1:/#; auto => />; rewrite ifF 1:/#; apply H5 => //.
+        * rewrite initiE 1:/#; auto => />; rewrite ifT 1:/# H9 1:/#; apply H6 => //.
+        * rewrite initiE 1:/#; auto => />; rewrite ifT 1:/# H9 1:/#; apply H7 => //.
+seq 2 0 : (
+  #pre /\
+  forall (k : int), 0 <= k < 32 => bufn1{1}.[k] = seed_p{1}.[64 + k]
+); first by auto => /> *; smt(@Array32).
+seq 1 0 : (#pre /\ bufn0{1} = bufn1{1}); first by ecall {1} (_x_memcpy_u8u8_post bufn1{1}); skip => />. 
+seq 1 0 : (
+  to_list seed_p{1} = sk_seed{2} ++ sk_prf{2} ++ pub_seed{2} /\
+  size sk_seed{2} = 32 /\
+  size sk_prf{2} = 32 /\
+  size pub_seed{2} = 32 /\
+  pk0{1} = pk{1} /\
+  seed0{1} = seed_p{1} /\
+  address{2} = top_tree_addr{1} /\
+
+  (forall (k : int), 0 <= k < 32 => seed_p{1}.[k] = nth witness sk_seed{2} k) /\
+  (forall (k : int), 0 <= k < 32 => seed_p{1}.[32 + k] = nth witness sk_prf{2} k) /\
+  (forall (k : int), 0 <= k < 32 => seed_p{1}.[64 + k] = nth witness pub_seed{2} k) /\
+
+  to_list idx{1} = nseq 4 W8.zero /\
+
+  (forall (k : int), 0 <= k < 4 => sk0{1}.[k] = W8.zero) /\
+  (forall (k : int), 0 <= k < 32 => sk0{1}.[4 + k] = nth witness sk_seed{2} k) /\
+  (forall (k : int), 0 <= k < 32 => sk0{1}.[4 + 32 + k] = nth witness sk_prf{2} k) /\
+  (forall (k : int), 0 <= k < 32 => sk0{1}.[4 + 3 * 32 + k] = nth witness pub_seed{2} k)
+).
+    + auto => /> &1 &2 H0 H1 H2 H3 H4 H5 H6 H7 H8 H9 H10 H11; do split => k??; rewrite initiE 1:/#; auto => />; first by smt(). 
+       * rewrite ifF 1:/# -H9 //=.  
+       * rewrite ifF 1:/# -H10 //=.
+       * rewrite ifT 1:/# -H6 //= H11 //=. 
+(* At this point, sk has all the fields set (except for the root) *)
 seq 2 0 : (
   #pre /\
   (forall (k : int), 0 <= k < 32 => bufn1{1}.[k] = sk0{1}.[100 + k]) 
 ); first by auto => /> *; rewrite initiE /#. 
 seq 1 0 : (#pre /\ bufn0{1} = bufn1{1}); first by ecall {1} (_x_memcpy_u8u8_post bufn1{1}); skip => />. 
+
 seq 1 0 : (
-  (* This is #pre but without the "pk0{1} = pk{1}" and the bufn parts *)
   to_list seed_p{1} = sk_seed{2} ++ sk_prf{2} ++ pub_seed{2} /\
   size sk_seed{2} = 32 /\
   size sk_prf{2} = 32 /\
   size pub_seed{2} = 32 /\
   seed0{1} = seed_p{1} /\
   address{2} = top_tree_addr{1} /\
+
+  (forall (k : int), 0 <= k < 32 => seed_p{1}.[k] = nth witness sk_seed{2} k) /\
+  (forall (k : int), 0 <= k < 32 => seed_p{1}.[32 + k] = nth witness sk_prf{2} k) /\
+  (forall (k : int), 0 <= k < 32 => seed_p{1}.[64 + k] = nth witness pub_seed{2} k) /\
+
   to_list idx{1} = nseq 4 W8.zero /\
+
+
   (forall (k : int), 0 <= k < 4 => sk0{1}.[k] = W8.zero) /\
-  (forall (k : int), 0 <= k < 64 => sk0{1}.[4 + k] = seed_p{1}.[k]) /\
-  (forall (k : int), 0 <= k < 32 => sk0{1}.[4 + 3 * 32 + k] = seed_p{1}.[64 + k]) /\
+  (forall (k : int), 0 <= k < 32 => sk0{1}.[4 + k] = nth witness sk_seed{2} k) /\
+  (forall (k : int), 0 <= k < 32 => sk0{1}.[4 + 32 + k] = nth witness sk_prf{2} k) /\
+  (forall (k : int), 0 <= k < 32 => sk0{1}.[4 + 3 * 32 + k] = nth witness pub_seed{2} k) /\
 
-  (* this is new *)
-  (forall (k : int), 0 <= k < 32 => pk0{1}.[32 + k] = sk0{1}.[100 + k])
-); first by auto => &1 &2; move => [#] *; do split; 1..10: assumption; move => k?; rewrite initiE /#. 
-seq 2 0 : (
-  (* buf0 = sk seed /\ buf1 = pub seed *)
-  #pre /\
-  (forall (k : int), 0 <= k < 32 => bufn0{1}.[k] = sk0{1}.[4 + k]) /\
-  (forall (k : int), 0 <= k < 32 => bufn1{1}.[k] = pk0{1}.[32 + k])
-); first by auto => /> &1 &2 *; split => *; rewrite initiE //=.
-
-seq 0 1 : (
-  #pre /\
-  toByte sk{2}.`idx 4 = sub sk0{1} 0  4  /\
-  sk{2}.`sk_seed      = sub sk0{1} 4  32 /\
-  sk{2}.`sk_prf       = sub sk0{1} 36 32 /\
-  sk{2}.`pub_seed_sk  = sub sk0{1} 68 32  
+  (forall (k : int), 0 <= k < 32 => pk0{1}.[32 + k] = nth witness pub_seed{2} k) (* this is the pub seed *)
 ).
-    + auto => /> &1 &2 H0 H1 H2 H3 H4 H5 H6 H7 H8 H9 H10; do split.
-           - rewrite toByteZero. apply (eq_from_nth witness).
-               * rewrite size_nseq size_sub /#.
-             rewrite size_nseq (: max 0 4 = 4) //=  => i Hi.
-             rewrite nth_nseq // nth_sub // /#.
-           - apply (eq_from_nth witness); first by rewrite H1 size_sub //=.
-             rewrite H1 => i Hi. 
-             rewrite nth_sub //= H6 1:/# -get_to_list H0 nth_cat !size_cat H1 H2 ifT 1:/#.
-             rewrite nth_cat H1 ifT 1:/# //=.
-           - apply (eq_from_nth witness); first by rewrite H2 size_sub //=.
-             rewrite H2 => i Hi. 
-             rewrite nth_sub //=.  
-             rewrite (nth_seed_1 (to_list seed_p{1}) sk_seed{2} sk_prf{2} pub_seed{2}) 1:/#.
-             rewrite get_to_list /#. 
-           - apply (eq_from_nth witness); first by rewrite H3 size_sub //=.
-             rewrite H3 => i Hi.
-             rewrite nth_sub 1:/#.
-             rewrite (nth_seed_2 (to_list seed_p{1}) sk_seed{2} sk_prf{2} pub_seed{2}) 1:/#.
-             rewrite get_to_list.  (* Isto esta certo mas a hipotese H7 devia ser falsa *)
-             admit.
+    + auto => /> &1 &2 H0 H1 H2 H3 H4 H5 H6 H7 H8 H9 H10 H11 H12 k ??.
+      rewrite initE ifT 1:/#; auto => />.
+      rewrite ifT 1:/# -H11 1:/# H12 //=.  
+seq 2 0 : (
+  #pre /\
+  to_list bufn0{1} = sk_seed{2} /\
+  to_list bufn1{1} = pub_seed{2}
+).
+    + auto => /> &1 &2 H0 H1 H2 H3 H4 H5 H6 H7 H8 H9 H10 H11 H12; split. 
+        - apply (eq_from_nth witness); [by rewrite size_to_list H1 | rewrite size_to_list => i?].
+          rewrite get_to_list initiE 1:/#; auto => />; rewrite -H9 //=.
+        - apply (eq_from_nth witness); [by rewrite size_to_list H3 | rewrite size_to_list => i?].
+          rewrite get_to_list initiE 1:/#; auto => />; rewrite H12 1:/# //=.
+seq 0 1 : (
+    #pre /\ 
+    toByte sk{2}.`idx 4 = sub sk0{1} 0  4  /\
+    sk{2}.`sk_seed      = sub sk0{1} 4  32 /\
+    sk{2}.`sk_prf       = sub sk0{1} 36 32 /\
+    sk{2}.`pub_seed_sk  = sub sk0{1} 100 32 (* NOTA: a pub seed e a root estao trocadas => Na spec a root vem no fim mas na impl no fim esta a pub seed => a root esta entre a sk prf e a pub seed *)
+).
+    + auto => /> &1 &2 H0 H1 H2 H3 H4 H5 H6 H7 H8 H9 H10 H11 H12; do split.
+      * apply (eq_from_nth witness); rewrite /toByte size_take //= size_rev size_to_list //=; [ by rewrite size_sub //= |] => i?. 
+        rewrite nth_sub //= nth_take //= 1:/# nth_rev 1:#smt:(size_to_list) size_to_list //=.
+        have ->: to_list (unpack8 W32.zero) = nseq 4 W8.zero.
+             - rewrite /unpack8. admit.
+        rewrite nth_nseq 1:/# H8 //=.    
+      * apply (eq_from_nth witness); [by rewrite size_to_list size_sub | rewrite size_to_list] => i?.
+        rewrite get_to_list nth_sub //= H9 //.
+      * apply (eq_from_nth witness); [by rewrite H2 size_sub | rewrite H2] => i?.
+        rewrite nth_sub //= H10 //.
+      * apply (eq_from_nth witness); [by rewrite size_to_list size_sub | rewrite size_to_list] => i?.
+        rewrite nth_sub //= -H11 //=.
 seq 1 1 : (#pre /\ root{2} = to_list root{1}).
     + admit.
-admit.
+seq 1 0  : (
+  #pre /\
+  (forall (k : int), 0 <= k < 32 => pk0{1}.[k] = nth witness root{2} k)
+).
+    + admit.
+seq 1 0 : (
+  #pre /\
+  (forall (k : int), 0 <= k < 32 => sk0{1}.[4 + 2 * 32 + k] = nth witness root{2} k)
+).
+    + admit.
+auto => /> &1 &2 H0 H1 H2 H3 H4 H5 H6 H7 H8 H9 H10 H11 H12 H13 H14 H15 H16 H17 H18; split. 
+    + admit.
+    + rewrite /DecodeSkNoOID => />. rewrite tP => i Hi. rewrite -!get_to_list.
+      case (0 <= i < 4); last by admit.
+        (* This case refers to the idx *)
+        + move => ?; 
+          rewrite of_listK; [by rewrite !size_cat !size_to_list H2 size_W32toBytes |].
+          do ! (rewrite nth_cat !size_cat !size_to_list H2 size_W32toBytes //= ifT 1:/#).
+          rewrite nth_cat !size_cat !size_to_list size_W32toBytes //= ifT 1:/#.
+          rewrite nth_cat size_W32toBytes ifT 1:/#.
 qed.
 
 
